theories/partial_function_test.v
@@ -1,0 +1,99 @@
+Require Import String.
+Require Import qterm.
+Require Import lambdaFacts.
+Require Import lambdaSolve.
+
+
+(*
+Can I define partial functions over lambda calculus terms with equations
+if I can prove that the inputs don't overlap?
+Or does it only work with elements of an inductive type?
+*)
+
+From Coq Require Import Arith Program.
+From Equations Require Import Equations.
+
+
+Equations neg (b : bool) : bool :=
+neg true := false ;
+neg false := true.
+
+Fail Equations test (t : QTerm) : nat :=
+  test (var "a"%string 0) := 0.
+
+
+
+(* No, it doesn't work. It wants a constructor. *)
+
+(*
+Maybe I can define my own way of defining partial functions?
+ *)
+
+Inductive Inhabited {T : Type} (set : T -> Prop) : Prop :=
+| squash : forall (t : T), set t -> Inhabited set
+.
+
+Record Partial (T : Type) : Type := {
+    elem : T -> Prop;
+    inhabited : Inhabited elem;
+    unique : forall t1 t2, elem t1 -> elem t2 -> t1 = t2
+  }.
+
+Theorem bind (A B : Type) (f : A -> Partial B) (a : Partial A) : Partial B.
+Proof.
+  refine {|
+      elem := fun b => forall x, elem _ a x -> elem _ (f x) b
+    ;
+      inhabited := _
+    ;
+      unique := _
+    |}.
+  (* inhabited *)
+  destruct (inhabited _ a).
+  destruct (inhabited _ (f t)).
+  eapply squash.
+  intros.
+  destruct (inhabited _ (f x)).
+  apply H2.
+  apply t0.
+  (* unique *)
+  intros.
+  destruct (inhabited _ a).
+  destruct (inhabited _ (f t)).
+  specialize (H t).
+  apply (unique (f x)).
+
+Theorem bind (A B : Type) (f : A -> Partial B) (a : Partial A) : Partial B.
+Proof. 
+  refine {|elem := _; unique := _|}.
+  Unshelve.
+  2: {
+    intro b.
+    Check (elem (f a)).
+    apply (elem f).
+    
+
+Record FunSpec (A B: Type) : Type := {
+    X : Type;
+    lhs : X -> A;
+    rhs : (A -> Partial B) -> X -> Partial B;
+    unique_lhs : forall a1 a2, lhs a1 = lhs a2 -> a1 = a2
+  }.
+
+(*
+Actually, there is no need for all that. It should be possible to just define:
+partialIf : Prop -> A -> A -> Partial A
+that just does "if" except with a proposition.
+Also, define
+fixpoint : (A -> Partial A) -> Partial A
+or maybe instead,
+fixpoint : ((A -> Partial B) -> A -> Partial B) -> A -> Partial B
+ *)
+
+Theorem propIf : forall A, Prop -> A -> A -> Partial A.
+Proof.
+
+Inductive Graph (A B : Type) (spec : FunSpec A B) : Prop :=
+| call : forall ,
+    
+.
